Update SEARrecsp.sml

SEARrecsp.sml
@@ -1,3 +1,139 @@
+
+val InjN_def = proved_th $
+e0
+(strip_tac >> irule
+ (P2fun_uex |> qspecl [‘N’,‘Pow(N * A)’] 
+ |> fVar_sInst_th “P(n0:mem(N),na:mem(Pow(N * A)))”
+    “(!n:mem(N) a:mem(A).IN(Pair(n,a),na) <=> n = n0)”) >>
+ strip_tac >> accept_tac
+ (IN_def_P |> qspecl [‘N * A’] 
+ |> fVar_sInst_th “P(na:mem(N * A))” “Fst(na:mem(N * A)) = x”
+ |> conv_rule (depth_fconv no_conv forall_cross_fconv)
+ |> rewr_rule[Pair_def'])
+)
+(form_goal “!A. ?!injN:N -> Pow(N * A).
+ !n0. (!n a.IN(Pair(n,a),App(injN,n0)) <=> n = n0)”)
+|> spec_all |> uex2ex_rule |> qSKOLEM "InjN" [‘A’] |> gen_all 
+
+
+val InjA_def = proved_th $
+e0
+(strip_tac >> irule
+ (P2fun_uex |> qspecl [‘A’,‘Pow(N * A)’] 
+ |> fVar_sInst_th “P(a0:mem(A),na:mem(Pow(N * A)))”
+    “(!n:mem(N) a:mem(A).IN(Pair(n,a),na) <=> a = a0)”) >>
+ strip_tac >> accept_tac
+ (IN_def_P |> qspecl [‘N * A’] 
+ |> fVar_sInst_th “P(na:mem(N * A))” “Snd(na:mem(N * A)) = x”
+ |> conv_rule (depth_fconv no_conv forall_cross_fconv)
+ |> rewr_rule[Pair_def']))
+(form_goal “!A. ?!injA:A -> Pow(N * A).
+ !a0. (!n a.IN(Pair(n,a),App(injA,a0)) <=> a = a0)”)
+|> spec_all |> uex2ex_rule |> qSKOLEM "InjA" [‘A’] |> gen_all 
+
+val Even_def = qdefine_psym("Even",[‘n:mem(N)’]) ‘∃n0. n = Mul(Suc(Suc(O)),n0)’
+val Odd_def = qdefine_psym("Odd",[‘n:mem(N)’]) ‘~Even(n)’
+
+
+(*pretend div2 is defined*)
+val Div2_def = qdefine_fsym("Div2",[‘n:mem(N)’]) ‘n’
+
+
+val num1_def = qdefine_fsym("num1",[]) ‘Suc(O)’
+val num2_def = qdefine_fsym("num2",[]) ‘Suc(num1)’
+val num3_def = qdefine_fsym("num3",[]) ‘Suc(num2)’
+val num4_def = qdefine_fsym("num4",[]) ‘Suc(num3)’
+
+
+                          
+val InjUU_def = proved_th $
+e0
+(strip_tac >> irule
+ (P2fun_uex |> qspecl [‘Pow(N * A) * Pow(N * A)’,‘Pow(N * A)’] 
+ |> fVar_sInst_th “P(u12:mem(Pow(N * A) * Pow(N * A)), s:mem(Pow(N * A)))”
+    “∀n a. IN(Pair(n,a),s:mem(Pow(N * A))) ⇔ 
+    ((Even(n) & IN(Pair(Div2(n),a),Fst(u12))) | 
+     (Odd(n) & IN(Pair(Div2(n),a),Snd(u12))))”
+ |> conv_rule (depth_fconv no_conv forall_cross_fconv)
+ |> rewr_rule[Pair_def']) >>
+ rpt strip_tac >> accept_tac
+ (IN_def_P |> qspecl [‘N * A’]
+ |> fVar_sInst_th “P(na:mem(N * A))”
+ “(Even(Fst(na)) & IN(Pair(Div2(Fst(na)),Snd(na)),a:mem(Pow(N * A)))) | 
+ (Odd(Fst(na)) & IN(Pair(Div2(Fst(na)),Snd(na)),b))”
+ |> conv_rule (depth_fconv no_conv forall_cross_fconv)
+ |> rewr_rule[Pair_def']))
+(form_goal “∀A.∃!f:Pow(N * A) * Pow(N * A) -> Pow(N * A).
+ ∀u1 u2. ∀n a. IN(Pair(n,a),App(f,Pair(u1,u2))) ⇔ 
+  ((Even(n) & IN(Pair(Div2(n),a),u1)) | 
+   (Odd(n) & IN(Pair(Div2(n),a),u2)))”)
+|> spec_all |> uex2ex_rule |> qSKOLEM "InjUU" [‘A’]
+
+val injUU_def = 
+    qdefine_fsym("injUU",[‘u1:mem(Pow(N * A))’,‘u2:mem(Pow(N * A))’]) 
+                ‘App(InjUU(A),Pair(u1,u2))’ 
+
+val Even_not_Odd = prove_store("Even_not_Odd",
+e0
+cheat
+(form_goal “!n. Even(n) <=> ~Odd(n)”));
+
+
+
+val Odd_not_Even = prove_store("Odd_not_Even",
+e0
+cheat
+(form_goal “!n. Odd(n) <=> ~Even(n)”));
+
+
+val injUU_char = prove_store("injUU_char",
+e0
+(rpt strip_tac (* 2 *)
+ >-- (rw[injUU_def,InjUU_def] >> arw[Odd_not_Even]) >> 
+ rw[injUU_def,InjUU_def] >> arw[Even_not_Odd])
+(form_goal “
+ (!n. Even(n) ==> (!A u1:mem(Pow(N * A)) u2 a. IN(Pair(n,a),injUU(u1,u2)) <=> IN(Pair(Div2(n),a),u1))) & 
+ (!n. Odd(n) ==> (!A u1:mem(Pow(N * A)) u2 a. IN(Pair(n,a),injUU(u1,u2)) <=> IN(Pair(Div2(n),a),u2)))”));
+
+val injUU_Even = injUU_char |> conjE1
+                            
+
+val InjUU_Inj = prove_store("InjUU_Inj",
+e0
+(strip_tac >> rw[Inj_def] >> rpt strip_tac >>
+ ccontra_tac >>
+ qsuff_tac ‘~(App(InjUU(A), x1) = App(InjUU(A), x2))’
+ >-- arw[] >>
+ last_x_assum (K all_tac) >>
+ qsspecl_then [‘x1’] (x_choosel_then ["u1","u2"] assume_tac) Pair_has_comp>>
+ qsspecl_then [‘x2’] (x_choosel_then ["u3","u4"] assume_tac) Pair_has_comp>>
+ fs[] >> fs[Pair_eq_eq] >> rw[GSYM injUU_def] >> 
+ qby_tac ‘~(u1 = u3) | ~(u2 = u4)’ >-- cheat >>
+ pop_assum strip_assume_tac >>
+ last_x_assum (K all_tac) (* 2 *)
+ >-- (fs[GSYM IN_EXT_iff] >> 
+     qby_tac ‘(?n a. IN(Pair(n,a),u1) & ~(IN(Pair(n,a),u3))) | 
+              (?n a. IN(Pair(n,a),u3) & ~(IN(Pair(n,a),u1)))’
+     >-- cheat >> pop_assum strip_assume_tac (* 2 *)
+     >-- (qsuff_tac
+         ‘?n a. IN(Pair(n,a),injUU(u1,u2)) & ~IN(Pair(n,a),injUU(u3,u4))’
+         >-- cheat >>
+         qexistsl_tac [‘Mul(num2,n)’,‘a’] >>
+         qby_tac ‘Even(Mul(num2,n))’ >-- cheat >>
+         drule injUU_Even >> arw[] >>
+         qby_tac ‘Div2(Mul(num2, n)) = n’ >-- cheat >> arw[])
+     >-- cheat (*same*)) >>
+ cheat)
+(form_goal “!A. Inj(InjUU(A))”));
+
+val injN_def = qdefine_fsym("injN",[‘A’,‘n:mem(N)’]) ‘App(InjN(A),n)’
+val injA_def = qdefine_fsym("injA",[‘a:mem(A)’]) ‘App(InjA(A),a)’ 
+
+
+
+
+
+
 val Lf0_def = qdefine_fsym("Lf0",[‘A’]) ‘injN(A,O)’
 
 (*
@@ -277,9 +413,622 @@ e0
  drule (Tind_rules |> conjE2 |> spec_all 
                    |> undisch |> gen_all
                    |> disch_all) >> 
- qexists_tac ‘Fnap(Fn, n, a, f, j)’ >> arw[]
+ qexists_tac ‘Fnap(Fn, n, a, f, j)’ >> arw[] >>
  rpt strip_tac >> drule $ iffLR Tind_cases >>
  fs[Pair_eq_eq,Nd_NONLF,Nd_eq_eq] >>
  qby_tac ‘y = j’ >>
  fs[] >> cheat)
 (form_goal “!X l:mem(X) A  Fn  t:mem(Tree(A)). ?!e. IN(Pair(t,e),Tinds(Fn,l))”));
+
+
+val Trec_def = P2fun' |> qspecl [‘Tree(A)’,‘X’] 
+                      |> fVar_sInst_th “P(t:mem(Tree(A)),
+                                          x:mem(X))”
+                          “IN(Pair(t:mem(Tree(A)),x),
+                              Tinds(Fn,l:mem(X)))”
+                      |> C mp (Tind_uex |> spec_all
+                                        |> qgen ‘t’)
+                      |> qSKOLEM "Trec" [‘Fn’,‘l’]
+                      |> qgenl [‘X’,‘l’,‘A’,‘Fn’]
+                      |> store_as "Trec_def";
+
+
+
+val Trec_Lf = prove_store("Trec_Lf",
+e0
+(rpt strip_tac >>
+ qsspecl_then [‘l’,‘Fn’,‘Lf(A)’] assume_tac Trec_def >>
+ drule $ iffLR Tind_cases >>
+ fs[Pair_eq_eq,GSYM Nd_NONLF])
+(form_goal “!X l:mem(X) A  Fn. 
+ App(Trec(Fn,l),Lf(A)) = l”));
+
+
+val App_Trec_Tinds = prove_store("App_Trec_Tinds",
+e0
+(rpt strip_tac >> dimp_tac >> strip_tac >--
+(pop_assum (assume_tac o GSYM) >> arw[Trec_def]) >>
+qsspecl_then [‘l’,‘Fn’,‘t’] assume_tac Trec_def >>
+qsspecl_then [‘l’,‘Fn’,‘t’] assume_tac Tind_uex >>
+pop_assum (strip_assume_tac o uex_expand) >>
+first_assum rev_drule >> arw[] >>
+first_assum irule >> arw[])
+(form_goal “!X l:mem(X) A  Fn.
+!t:mem(Tree(A)) x. App(Trec(Fn,l),t) = x <=> 
+IN(Pair(t,x),Tinds(Fn,l))”));
+
+
+val Trec_Nd = prove_store("Trec_Nd",
+e0
+(rpt strip_tac >>
+ qsspecl_then [‘l’,‘Fn’,‘Nd(n,a,f)’] assume_tac Trec_def >>
+ drule $ iffLR Tind_cases >> 
+ fs[Pair_eq_eq,Nd_NONLF,Nd_eq_eq] >>
+ qsuff_tac ‘y = Trec(Fn, l) o f'’ 
+ >-- (strip_tac >> arw[]) >>
+ flip_tac >> irule $ iffLR FUN_EXT >>
+ rw[App_App_o] >>  arw[App_Trec_Tinds])
+(form_goal “!X l:mem(X) A  Fn n a:mem(A) f. 
+ App(Trec(Fn,l),Nd(n,a,f)) = 
+ Fnap(Fn,n,a,f,Trec(Fn,l) o f)”));
+
+
+val TNull_def = proved_th $
+e0
+cheat
+(form_goal “!A. ?!f:N->Tree(A). !n. App(f,n) = Lf(A)”)
+|> spec_all |> uex2ex_rule |> qSKOLEM "TNull" [‘A’]
+
+val Bot0_def = qdefine_fsym("Bot0",[‘A’])
+‘Nd(O,NONE(A),TNull(A+1))’
+
+
+val Var0_def = qdefine_fsym("Var0",[‘a:mem(A)’])
+‘Nd(num1,SOME(a),TNull(A+1))’
+
+
+val T1arg_def = 
+proved_th $
+e0
+cheat
+(form_goal “!A t. ?!f:N->Tree(A). 
+ App(f,O) = t & 
+!n. App(f,Suc(n)) = Lf(A)”)
+|> spec_all |> uex2ex_rule |> qSKOLEM "T1arg" [‘t’]
+
+val Neg0_def = qdefine_fsym("Neg0",[‘f:mem(Tree(A + 1))’])
+‘Nd(num2,NONE(A),T1arg(f))’
+
+
+
+val T2arg_def = 
+proved_th $
+e0
+cheat
+(form_goal “!A t1 t2. ?!f:N->Tree(A). 
+ App(f,O) = t1 & 
+ App(f,num1) = t2 &
+ (!n. ~(n = O) & ~(n = num1) ==> App(f,n) = Lf(A))”)
+|> spec_all |> uex2ex_rule |> qSKOLEM "T2arg" [‘t1’,‘t2’]
+
+
+val Disj0_def = qdefine_fsym("Disj0",[‘f1:mem(Tree(A + 1))’,
+                                      ‘f2:mem(Tree(A + 1))’])
+‘Nd(num3,NONE(A),T2arg(f1,f2))’
+
+val Diam0_def = qdefine_fsym("Diam0",[‘f:mem(Tree(A + 1))’])
+‘Nd(num4,NONE(A),T1arg(f))’
+
+(*
+val X1arg_def = 
+proved_th $
+e0
+cheat
+(form_goal “!X x. ?!f:N->X+1. 
+ App(f,O) = SOME(x) & 
+!n. App(f,Suc(n)) = NONE(X)”)
+|> spec_all |> uex2ex_rule |> qSKOLEM "X1arg" [‘x’]
+
+val X2arg_def = 
+proved_th $
+e0
+cheat
+(form_goal “!X x1 x2. ?!f:N->X + 1. 
+ App(f,O) = SOME(x1) & 
+ App(f,num1) = SOME(x2) &
+ (!n. ~(n = O) & ~(n = num1) ==> App(f,n) = NONE(X))”)
+|> spec_all |> uex2ex_rule |> qSKOLEM "X2arg" [‘x1’,‘x2’]
+
+
+val fmFn_def = proved_th $
+e0
+cheat
+(form_goal
+ “!X x0:mem(X) A vf:A->X nf:X->X djf:X*X->X dmf:X->X.
+  ?!Fn:N * (A + 1) * Exp(N,Tree(A+1)) * Exp(N,X+1) -> X+1.
+  Fnap(Fn,O,NONE(A),TNull(A+1),Null(X)) = SOME(x0) &
+  (!a. Fnap(Fn,num1,SOME(a),TNull(A+1),Null(X)) = 
+       SOME(App(vf,a))) &
+  (!f0 x. Fnap(Fn,num2,NONE(A),T1arg(f0),X1arg(x)) = 
+       SOME(App(nf,x))) & 
+  (!f1 f2 x1 x2. 
+    Fnap(Fn,num3,NONE(A),T2arg(f1,f2),X2arg(x1,x2)) = 
+    SOME(App(djf,Pair(x1,x2)))) &
+  (!f0 x. Fnap(Fn,num4,NONE(A),T1arg(f0),X1arg(x)) = 
+       SOME(App(dmf,x))) ”)
+|> spec_all |> uex2ex_rule |> qSKOLEM "fmFn" [‘x0’,‘vf’,‘nf’,‘djf’,‘dmf’]
+*)
+
+(*constant at*)
+val Conat_def = proved_th $
+e0
+cheat
+(form_goal “!X x:mem(X). ?!f:N->X.!n.App(f,n) = x”)
+|> spec_all |> uex2ex_rule |> qSKOLEM "Conat" [‘x’]
+
+
+val X1arg_def = 
+proved_th $
+e0
+cheat
+(form_goal “!X x x0. ?!f:N->X. 
+ App(f,O) = x & 
+!n. App(f,Suc(n)) = x0”)
+|> spec_all |> uex2ex_rule |> qSKOLEM "X1arg" [‘x’,‘x0’]
+
+val X2arg_def = 
+proved_th $
+e0
+cheat
+(form_goal “!X x1 x2 x0. ?!f:N->X. 
+ App(f,O) = x1 & 
+ App(f,num1) = x2 &
+ (!n. ~(n = O) & ~(n = num1) ==> App(f,n) = x0)”)
+|> spec_all |> uex2ex_rule |> qSKOLEM "X2arg" [‘x1’,‘x2’,‘x0’]
+
+
+val fmFn_def = proved_th $
+e0
+cheat
+(form_goal
+ “!X x0:mem(X) A vf:A->X nf:X->X djf:X*X->X dmf:X->X.
+  ?!Fn:N * (A + 1) * Exp(N,Tree(A+1)) * Exp(N,X) -> X.
+  Fnap(Fn,O,NONE(A),TNull(A+1),Conat(x0)) = x0 &
+  (!a. Fnap(Fn,num1,SOME(a),TNull(A+1),Conat(x0)) = 
+       App(vf,a)) &
+  (!f0 x. Fnap(Fn,num2,NONE(A),T1arg(f0),X1arg(x,x0)) = 
+   App(nf,x)) & 
+  (!f1 f2 x1 x2. 
+    Fnap(Fn,num3,NONE(A),T2arg(f1,f2),X2arg(x1,x2,x0)) = 
+       App(djf,Pair(x1,x2))) &
+  (!f0 x. Fnap(Fn,num4,NONE(A),T1arg(f0),X1arg(x,x0)) = 
+       App(dmf,x))  ”)
+|> spec_all |> uex2ex_rule |> qSKOLEM "fmFn" [‘x0’,‘vf’,‘nf’,‘djf’,‘dmf’]
+
+
+
+
+val rec_NONE_TNull_Conat= prove_store("rec_NONE_TNull_Conat",
+e0
+(rw[GSYM FUN_EXT,App_App_o,TNull_def,Trec_Lf,Null_def,Conat_def])
+(form_goal
+“!A X f x0:mem(X).Trec(f, x0) o TNull(A + 1) = Conat(x0)”));
+
+
+val Bot0_x0 = 
+Trec_Nd |> qspecl [‘X’,‘x0:mem(X)’,‘A+1’,‘fmFn(x0:mem(X),vf:A->X,nf,djf,dmf)’,‘O’,‘NONE(A)’,‘TNull(A+1)’]
+|> rewr_rule[GSYM Bot0_def,fmFn_def,rec_NONE_TNull_Conat]
+
+val Var0_vf = 
+Trec_Nd |> qspecl [‘X’,‘x0:mem(X)’,‘A+1’,‘fmFn(x0:mem(X),vf:A->X,nf,djf,dmf)’,‘num1’,‘SOME(a:mem(A))’,‘TNull(A+1)’]
+|> rewr_rule[GSYM Var0_def,fmFn_def,rec_NONE_TNull_Conat]
+
+
+val Fnap_Neg0 = fmFn_def |> conjE2 |> conjE2 |> conjE1
+
+
+val rec_NONE_T1arg_X1arg= prove_store("rec_NONE_T1arg_X1arg",
+e0
+(rw[GSYM FUN_EXT,App_App_o,TNull_def,Trec_Lf] >>
+ strip_tac >>
+ qcases ‘a = O’ 
+ >-- arw[X1arg_def,T1arg_def] >>
+ fs[O_xor_Suc,T1arg_def,X1arg_def,Trec_Lf] )
+(form_goal
+“Trec(Fn, x0:mem(X)) o T1arg(f0:mem(Tree(A))) = 
+ X1arg(App(Trec(Fn, x0),f0),x0)”));
+
+
+
+
+val Neg0_nf = 
+Trec_Nd |> qspecl [‘X’,‘x0:mem(X)’,‘A+1’,‘fmFn(x0:mem(X),vf:A->X,nf,djf,dmf)’,‘num2’,‘NONE(A)’,‘T1arg(f0:mem(Tree(A+1)))’]
+|> rewr_rule[GSYM Neg0_def,rec_NONE_T1arg_X1arg,Fnap_Neg0]
+
+
+val Diam0_dmf = 
+Trec_Nd |> qspecl [‘X’,‘x0:mem(X)’,‘A+1’,‘fmFn(x0:mem(X),vf:A->X,nf,djf,dmf)’,‘num4’,‘NONE(A)’,‘T1arg(f0:mem(Tree(A+1)))’]
+|> rewr_rule[GSYM Diam0_def,rec_NONE_T1arg_X1arg,fmFn_def]
+
+
+
+val Fnap_Disj0 = fmFn_def |> conjE2 |> conjE2 |> conjE2
+                          |> conjE1
+
+
+
+val rec_NONE_T2arg_X2arg = prove_store("rec_NONE_T2arg_X2arg",
+e0
+(rw[GSYM FUN_EXT,App_App_o,TNull_def,Trec_Lf] >>
+ strip_tac >>
+ qcases ‘a = O’ 
+ >-- arw[X2arg_def,T2arg_def] >>
+ qcases ‘a = num1’ 
+ >-- arw[X2arg_def,T2arg_def] >>
+ assume_tac (gen_all T2arg_def) >>
+ assume_tac (gen_all X2arg_def) >>
+ qby_tac ‘ App(T2arg(f1, f2), a) = Lf(A)’ 
+ >-- (first_x_assum (qsspecl_then [‘f1’,‘f2’] 
+                                 strip_assume_tac) >>
+     first_x_assum irule >> arw[]) >>
+ arw[Trec_Lf] >>flip_tac >> 
+ first_x_assum (qsspecl_then [‘x0’,‘App(Trec(Fn, x0), f1)’,‘App(Trec(Fn, x0), f2)’] 
+                                 strip_assume_tac) >>
+ first_x_assum irule >> arw[])
+(form_goal
+“Trec(Fn, x0:mem(X)) o T2arg(f1:mem(Tree(A)),f2) = 
+ X2arg(App(Trec(Fn, x0),f1),App(Trec(Fn, x0),f2),x0)”));
+
+val Disj0_djf = 
+Trec_Nd |> qspecl [‘X’,‘x0:mem(X)’,‘A+1’,‘fmFn(x0:mem(X),vf:A->X,nf,djf,dmf)’,‘num3’,‘NONE(A)’,‘T2arg(f1:mem(Tree(A+1)),f2)’]
+|> rewr_rule[GSYM Disj0_def,rec_NONE_T2arg_X2arg,fmFn_def]
+
+
+
+
+
+
+val isfm_cl = 
+  “(nas = Bot0(A) ==> IN(nas,isfms)) &
+  (!p:mem(A). nas = Var0(p) ⇒ IN(nas,isfms)) &
+  (∀f0.IN(f0,isfms) & nas = Neg0(f0) ⇒ IN(nas,isfms)) & 
+  (∀f1 f2.IN(f1,isfms) & IN(f2,isfms) & nas = Disj0(f1,f2) ⇒ IN(nas,isfms)) &
+  (∀f0.IN(f0,isfms) & nas = Diam0(f0) ⇒ IN(nas,isfms))”
+
+val (isfm_incond,x1) = mk_incond isfm_cl;
+val isfmf_ex = mk_fex isfm_incond x1;
+val isfmf_def = mk_fdef "isfmf" isfmf_ex;
+val isfmf_monotone = mk_monotone isfmf_def;
+val isfm's_def = mk_prim isfmf_def;
+val isfms_def = mk_LFP (rastt "isfm's(A)");
+val isfms_cond = mk_cond isfms_def isfm's_def;
+val isfms_SS = mk_SS isfms_def isfm's_def;
+val isfm_rules0 = mk_rules isfmf_monotone isfms_SS isfms_cond;
+val isfm_cases0 = mk_cases isfmf_monotone isfm_rules0 isfms_cond;
+val isfm_ind0 = mk_ind isfms_cond;
+val isfm_ind1 = mk_ind1 isfmf_def isfm_ind0;
+val isfm_ind2 = mk_ind2 isfm_ind1;
+val isfm_cases1 = mk_case1 isfmf_def isfm_cases0;
+val isfm_rules1 = mk_rules1 isfmf_def isfm_rules0;
+val isfm_rules2 = mk_rules2 isfm_rules1;
+val isfm_rules3 = mk_rules3 isfm_rules2;
+
+
+
+
+val isfm_ind = isfm_ind2 |> store_as "isfm_ind";
+val isfm_cases = isfm_cases1 |> store_as "isfm_cases";
+val isfm_rules = isfm_rules3 |> store_as "isfm_rules";
+
+
+val isfm_def = qdefine_psym("isfm",[‘f:mem(Tree(A+1))’])
+‘IN(f,isfms(A))’ |> gen_all 
+
+val form_def = Thm_2_4  |> qspecl [‘Tree(A+1)’]
+                        |> fVar_sInst_th “P(f:mem(Tree(A+1)))”
+                        “isfm(f:mem(Tree(A+1)))”
+                        |> qSKOLEM "form" [‘A’]
+                        |> qSKOLEM "repf" [‘A’]
+
+val isfm_clauses = isfm_rules |> rewr_rule[GSYM isfm_def]
+
+
+val isfm_induct = prove_store("isfm_induct",
+e0
+(rw[isfm_def] >> strip_tac >>
+ x_choose_then "s" (assume_tac o conjE1) 
+ (IN_def_P_expand |> qspecl [‘Tree(A+1)’]) >> arw[] >>
+ rpt strip_tac >> irule isfm_ind >> arw[])
+(form_goal 
+ “!A.P(Bot0(A)) & 
+  (!p:mem(A). P(Var0(p))) & 
+  (!f0:mem(Tree(A + 1)). P(f0) ==> P(Neg0(f0))) &
+  (!f1:mem(Tree(A + 1)) f2. P(f1) & P(f2) ==> P(Disj0(f1,f2))) &
+  (!f0:mem(Tree(A + 1)). P(f0) ==> P(Diam0(f0))) ==>
+  !f0:mem(Tree(A + 1)). isfm(f0) ==> P(f0)”));
+
+
+val Repf_def = qdefine_fsym("Repf",[‘f:mem(form(A))’]) ‘App(repf(A),f)’
+                           |> gen_all 
+
+
+val repf_Inj = form_def |> conjE1 |> store_as "repf_Inj";
+
+val Bot_def = proved_th $
+e0
+(rw[Repf_def] >> assume_tac repf_Inj >>
+ assume_tac Inj_ex_uex >>
+ first_x_assum (qsspecl_then [‘repf(A)’] assume_tac) >>
+ rfs[] >> 
+ flip_tac >> rw[GSYM form_def] >> rw[isfm_clauses])
+(form_goal “?!f. Repf(f) = Bot0(A)”)
+|> uex2ex_rule |> qSKOLEM "Bot" [‘A’]
+
+
+val VAR0_def = fun_tm_compr (dest_var (rastt "a:mem(A)")) (rastt "Var0(a:mem(A))")
+                            |> qSKOLEM "VAR0" [‘A’]
+
+
+val NEG0_def = fun_tm_compr (dest_var (rastt "t:mem(Tree(A+1))")) (rastt "Neg0(t:mem(Tree(A+1)))")
+                            |> qSKOLEM "NEG0" [‘A’]
+
+
+val DIAM0_def = fun_tm_compr (dest_var (rastt "t:mem(Tree(A+1))")) (rastt "Diam0(t:mem(Tree(A+1)))")
+                            |> qSKOLEM "DIAM0" [‘A’]
+
+
+val DISJ0_def = fun_tm_compr (dest_var (rastt "t12:mem(Tree(A+1) * Tree(A+1))")) (rastt "Disj0(Fst(t12:mem(Tree(A+1) * Tree(A+1))), Snd(t12:mem(Tree(A+1) * Tree(A+1))))")
+                            |> qSKOLEM "DISJ0" [‘A’]
+                            |> qspecl [‘Pair(t1:mem(Tree(A+1)),t2:mem(Tree(A+1)))’]
+                            |> rewr_rule[Pair_def']
+
+val DISJ0_Inj = prove_store("DISJ0_Inj",
+e0
+cheat
+(form_goal “Inj(DISJ0(A))”));
+
+val NEG0_Inj = prove_store("NEG0_Inj",
+e0
+cheat
+(form_goal “Inj(NEG0(A))”));
+
+
+val DIAM0_Inj = prove_store("DIAM0_Inj",
+e0
+cheat
+(form_goal “Inj(NEG0(A))”));
+
+
+val VAR0_Inj = prove_store("VAR0_Inj",
+e0
+cheat
+(form_goal “Inj(VAR0(A))”));
+
+val VAR_def = Inj_lift_fun |> qsspecl [‘repf(A)’]
+                           |> C mp repf_Inj
+                           |> qsspecl [‘VAR0(A)’] 
+                           |> rewr_rule[VAR0_def,GSYM form_def,
+                                        isfm_clauses]
+                           |> qSKOLEM "VAR" [‘A’]
+                           |> rewr_rule[App_App_o,GSYM Repf_def]
+
+val Var_def = qdefine_fsym("Var",[‘a:mem(A)’]) ‘App(VAR(A),a)’
+
+
+val repf_isfm = prove_store("repf_isfm",
+e0
+(rw[form_def] >> rpt strip_tac >> rw[Repf_def] >>
+ qexists_tac ‘f0’ >> rw[])
+(form_goal “!f0:mem(form(A)).isfm(Repf(f0))”));
+
+val isfm_Neg0 = isfm_clauses |> conjE2 |> conjE2 |> conjE1
+
+val isfm_Diam0 = isfm_clauses |> conjE2 |> conjE2 |> conjE2
+                              |> conjE2
+
+val isfm_Disj0 = isfm_clauses |> conjE2 |> conjE2 |> conjE2
+                              |> conjE1
+
+val Neg0_Repf = proved_th $
+e0
+(strip_tac >> irule isfm_Neg0 >> rw[repf_isfm])
+(form_goal “!f0:mem(form(A)). isfm(Neg0(Repf(f0)))”)
+
+
+val Diam0_Repf = proved_th $
+e0
+(strip_tac >> irule isfm_Diam0 >> rw[repf_isfm])
+(form_goal “!f0:mem(form(A)). isfm(Diam0(Repf(f0)))”)
+
+val Disj0_Repf = proved_th $
+e0
+(rpt strip_tac >> irule isfm_Disj0 >> rw[repf_isfm])
+(form_goal “!a b:mem(form(A)).isfm(Disj0(Repf(a), Repf(b)))”)
+
+
+val NEG_def = Inj_lift_fun_lemma |> qsspecl [‘repf(A)’]
+                           |> C mp repf_Inj
+                           |> qsspecl [‘NEG0(A)’] 
+                           |> rewr_rule[App_App_o,NEG0_def]
+                           |> rewr_rule[GSYM form_def,GSYM Repf_def]
+                           |> rewr_rule[Neg0_Repf]
+                           |> qSKOLEM "NEG" [‘A’]
+
+val DIAM_def = Inj_lift_fun_lemma |> qsspecl [‘repf(A)’]
+                           |> C mp repf_Inj
+                           |> qsspecl [‘DIAM0(A)’] 
+                           |> rewr_rule[App_App_o,DIAM0_def]
+                           |> rewr_rule[GSYM form_def,GSYM Repf_def]
+                           |> rewr_rule[Diam0_Repf]
+                           |> qSKOLEM "DIAM" [‘A’]
+
+
+val form_def_uex = prove_store("form_def_uex",
+e0
+(strip_tac >> assume_tac repf_Inj >>
+ drule Inj_ex_uex >> flip_tac >>
+ rw[Repf_def] >> arw[] >>
+ rw[form_def] >> lflip_tac >> rw[])
+(form_goal “!a:mem(Tree(A+1)).
+ (?!b. a = Repf(b)) <=> isfm(a)”));
+
+val DISJ_def = Inj_restrict |> qsspecl [‘Prla(repf(A),repf(A))’]
+                            |> C mp (Prla_Inj |> qsspecl [‘repf(A)’]
+                                              |> C mp repf_Inj
+                                              |> qsspecl [‘repf(A)’]
+                                              |> C mp repf_Inj)
+                            |> qsspecl [‘repf(A)’] 
+                            |> conv_rule
+                            (depth_fconv no_conv forall_cross_fconv)
+                            |> C mp repf_Inj
+                            |> qspecl [‘DISJ0(A)’]
+                            |> rewr_rule[App_App_o,Prla_def,App_Pa_Pair]
+                            |> rewr_rule[Pair_def,GSYM Repf_def]
+                            |> rewr_rule[form_def_uex,DISJ0_def,Pair_def']
+                            |> C mp Disj0_Repf
+                            |> uex2ex_rule
+                            |> qSKOLEM "DISJ" [‘A’] 
+                            |> rewr_rule[GSYM FUN_EXT] 
+                            |>  conv_rule
+                            (depth_fconv no_conv forall_cross_fconv)
+                            |> rewr_rule[App_App_o,App_Pa_Pair,Pair_def,
+                                         DISJ0_def,GSYM Repf_def] |> rewr_rule[Pair_def']
+
+val Neg_def = qdefine_fsym("Neg",[‘f:mem(form(A))’]) ‘App(NEG(A),f)’
+
+
+val Diam_def = qdefine_fsym("Diam",[‘f:mem(form(A))’]) ‘App(DIAM(A),f)’
+
+
+val Disj_def = qdefine_fsym("Disj",[‘f1:mem(form(A))’,‘f2:mem(form(A))’]) ‘App(DISJ(A),Pair(f1,f2))’
+
+
+val fmrec_def = qdefine_fsym("fmrec",[‘x0:mem(X)’,‘vf:A->X’,‘nf:X->X’,‘djf:X*X->X’,‘dmf:X->X’])
+‘Trec(fmFn(x0:mem(X), vf:A->X, nf, djf, dmf), x0) o repf(A)’
+
+
+
+val fmrec_clauses = prove_store("fmrec_clauses",
+e0
+(rpt strip_tac (* 5*) 
+ >-- rw[fmrec_def,App_App_o,Bot_def,GSYM Repf_def,
+        Bot0_x0]
+ >-- rw[fmrec_def,App_App_o,Var_def,VAR_def,GSYM Repf_def,
+        Var0_vf]
+ >-- rw[fmrec_def,App_App_o,Neg_def,NEG_def,GSYM Repf_def,
+        Neg0_nf]
+ >-- rw[fmrec_def,App_App_o,Disj_def,DISJ_def,GSYM Repf_def,
+        Disj0_djf]
+ >-- rw[fmrec_def,App_App_o,Diam_def,DIAM_def,GSYM Repf_def,
+        Diam0_dmf])
+(form_goal “!X x0 A vf:A->X nf djf:X * X->X dmf. 
+ App(fmrec(x0,vf,nf,djf,dmf),Bot(A)) = x0 & 
+ (!p.App(fmrec(x0,vf,nf,djf,dmf),Var(p)) = App(vf,p)) &
+ (!f.App(fmrec(x0,vf,nf,djf,dmf),Neg(f)) = 
+     App(nf,App(fmrec(x0,vf,nf,djf,dmf),f))) & 
+ (!f1 f2.App(fmrec(x0,vf,nf,djf,dmf),Disj(f1,f2)) = 
+     App(djf,Pair(App(fmrec(x0,vf,nf,djf,dmf),f1),
+                  App(fmrec(x0,vf,nf,djf,dmf),f2)))) & 
+ (!f.App(fmrec(x0,vf,nf,djf,dmf),Diam(f)) = 
+     App(dmf,App(fmrec(x0,vf,nf,djf,dmf),f))) ”));
+
+
+val form_def' = form_def |> conv_rule flip_fconv
+
+val form_induct = prove_store("form_induct",
+e0
+(strip_tac >> disch_tac >>
+ qsuff_tac ‘!f0:mem(Tree(A+1)). isfm(f0) ==> isfm(f0) &
+ !f.Repf(f) = f0 ==> P(f)’ 
+ >-- (strip_tac >>
+     qby_tac ‘!f0:mem(Tree(A+1)). isfm(f0) ==>
+                      (!f. Repf(f) = f0 ==> P(f))’ 
+     >-- (rpt strip_tac >> first_x_assum drule >>
+          rfs[] >> first_x_assum irule >> arw[]) >>
+     strip_tac >> first_x_assum irule >>
+     qexists_tac ‘Repf(f0)’ >> rw[repf_isfm]) >>
+ ind_with (isfm_induct |> qspecl [‘A’]) >>
+ rw[isfm_clauses] >> strip_tac (* 2 *)
+ >-- (rpt strip_tac >>
+     qsuff_tac ‘f = Bot(A)’ >-- (strip_tac >> arw[]) >>
+     irule $ iffLR Inj_eq_eq >> qexistsl_tac [‘Tree(A+1)’,‘repf(A)’] >>
+     arw[repf_Inj,Bot_def,GSYM Repf_def]) >> strip_tac (* 2 *)
+ >-- (rpt strip_tac >> 
+      qsuff_tac ‘f = Var(p)’ >-- (strip_tac >> arw[]) >>
+      irule $ iffLR Inj_eq_eq >> qexistsl_tac [‘Tree(A+1)’,‘repf(A)’] >>
+      arw[repf_Inj,Var_def,GSYM Repf_def,GSYM VAR_def,App_App_o]) >> 
+ strip_tac (* 2 *)
+ >-- (rpt gen_tac >> disch_tac >> 
+     pop_assum strip_assume_tac >> 
+     qby_tac ‘isfm(Neg0(f0))’ >-- (irule isfm_Neg0 >> arw[]) >> arw[] >>
+     rpt strip_tac >>
+     qby_tac ‘?f1. Repf(f1) = f0’ 
+     >-- arw[GSYM form_def',Repf_def] >>
+     pop_assum strip_assume_tac >> 
+     first_x_assum drule >>
+     fs[] >> 
+     qsuff_tac ‘f = Neg(f1)’ 
+     >-- (strip_tac >> arw[] >> first_x_assum irule >> arw[]) >>
+     rw[GSYM Repf_eq_eq] >> arw[Neg_def,NEG_def] >>
+      arw[]) >> strip_tac (* 2 *)
+>-- (rpt gen_tac >> disch_tac >> pop_assum strip_assume_tac >>
+    qby_tac ‘isfm(Disj0(f1, f2))’ 
+    >-- (irule isfm_Disj0 >> arw[]) >>
+    arw[] >> rpt strip_tac >> 
+    qby_tac ‘?f10. Repf(f10) = f1’ 
+    >-- arw[GSYM form_def',Repf_def] >>
+    pop_assum strip_assume_tac >> 
+    qby_tac ‘?f20. Repf(f20) = f2’ 
+    >-- arw[GSYM form_def',Repf_def] >>
+    pop_assum strip_assume_tac >> 
+    first_x_assum drule >> first_x_assum drule >> fs[] >>
+    qsuff_tac ‘f = Disj(f10,f20)’ 
+    >-- (rpt strip_tac >> arw[] >> first_x_assum irule >> arw[]) >>
+    rw[GSYM Repf_eq_eq] >> arw[Disj_def,DISJ_def]) >>
+rpt gen_tac >> disch_tac >> 
+pop_assum strip_assume_tac >> 
+qby_tac ‘isfm(Diam0(f0))’ >-- (irule isfm_Diam0 >> arw[]) >> arw[] >>
+rpt strip_tac >>
+qby_tac ‘?f1. Repf(f1) = f0’ 
+>-- arw[GSYM form_def',Repf_def] >>
+pop_assum strip_assume_tac >> 
+first_x_assum drule >>
+fs[] >> 
+qsuff_tac ‘f = Diam(f1)’ 
+>-- (strip_tac >> arw[] >> first_x_assum irule >> arw[]) >>
+rw[GSYM Repf_eq_eq] >> arw[Diam_def,DIAM_def])
+(form_goal
+ “!A.P(Bot(A)) & 
+  (!p:mem(A). P(Var(p))) & 
+  (!f0:mem(form(A)). P(f0) ==> P(Neg(f0))) &
+  (!f1:mem(form(A)) f2. P(f1) & P(f2) ==> P(Disj(f1,f2))) &
+  (!f0:mem(form(A)). P(f0) ==> P(Diam(f0))) ==>
+  !f0:mem(form(A)). P(f0)”));
+
+
+
+
+
+local 
+val l = proved_th $
+e0
+()
+(form_goal “”)
+Inj_restrict |> qsspecl [‘repf(A)’]
+|> rewr_rule[repf_Inj]
+|> qsspecl [‘Id(X)’]
+|> rewr_rule[Id_Inj,Id_def]
+|> qspecl [‘Trec(fmFn(x0:mem(X), vf:A->X, nf, djf, dmf), x0)’]
+|> rewr_rule[App_App_o,GSYM Repf_def,IdL]
+
+(*
+Vars are 
+Nd(0,NONE(A),(\n. Lf(A+1)))
+
+Fn: N -> A -> (N -> Tree(A)) -> (N -> X) -> X
+
+Fn: N -> A +1 -> (N -> Tree(A+1)) -> (N -> X) -> X
+
+Fn: N -> A+1 -> (N -> Tree(A) * X + 1) -> X
+
+*)
